Initial version of parallel reduce

src/examples/GPU.DotProduct2.fst
@@ -5,186 +5,420 @@ open Pulse.Lib.Array
 open Pulse.Lib.Pervasives
 module A = Pulse.Lib.Array
 module SZ = FStar.SizeT
+module U64 = FStar.UInt64
 open Pulse.Lib.BigStar
 open GPU
 
 let size : nat = 1024
 
-let kpre (ga1 ga2 r : gpu_array int size) (nth : nat) (tid:nat{tid < nth}) : slprop =
-  (gpu_pts_to_array1 ga1 tid **
-  gpu_pts_to_array1 ga2 tid) **
-  gpu_pts_to_array1 r tid
+let dot (s1 s2: erased (FStar.Seq.seq U64.t)) (#_: squash (FStar.Seq.length s1 == FStar.Seq.length s2)): erased (FStar.Seq.seq U64.t)
+  = FStar.Seq.init_ghost (FStar.Seq.length s1) (fun i -> U64.mul_mod (FStar.Seq.index s1 i) (FStar.Seq.index s2 i))
 
-let kpost (ga1 ga2 r : gpu_array int size) (nth : nat) (tid:nat{tid < nth}) : slprop =
-  (gpu_pts_to_array1 ga1 tid **
-  gpu_pts_to_array1 ga2 tid) **
-  gpu_pts_to_array1 r tid
+let rec log2 (n: nat{n <> 0}): (r:nat{r < n}) = if n = 1 then 0 else 1 + log2 (n / 2)
+let rec pow_log_lemma (n: nat): Lemma (log2 (pow2 n) = n) = if n = 0 then () else pow_log_lemma (n - 1)
+
+let div_pow_2 (i tid: nat): bool = tid % pow2 i = 0
+
+let mod_lemma (a b: nat):
+  Lemma (requires a < b) (ensures (a % b == a)) = ()
+
+let rec div_pow_2_lemma (i j tid: nat):
+  Lemma
+    (requires i < j)
+    (ensures (div_pow_2 j tid) ==> (div_pow_2 i tid))
+  = if not (div_pow_2 j tid) then () else (
+      if i = j - 1 then () else div_pow_2_lemma i (j - 1) tid;
+      // TODO:
+      assert (tid % (2 * pow2 (j - 1)) = 0);
+      assume (tid % pow2 (j - 1) = 0))
+
+let min (a b: nat): nat = if a < b then a else b
+
+// Pure SUM
+
+let rec sum_seq (s: FStar.Seq.seq U64.t) (i j:nat) (#_: squash (i < j && j <= FStar.Seq.length s)): Tot U64.t (decreases j - i) =
+  if i = j - 1 then FStar.Seq.index s i else U64.add_mod (FStar.Seq.index s i) (sum_seq s (i + 1) j)
+
+let add_mod_assoc (a b c: U64.t): Lemma (U64.add_mod (U64.add_mod a b) c = U64.add_mod a (U64.add_mod b c)) = admit()
+
+let rec sum_seq_lemma (s: FStar.Seq.seq U64.t) (i j k:nat):
+  Lemma (requires i < j && j < k && k <= FStar.Seq.length s) (ensures sum_seq s i k = U64.add_mod (sum_seq s i j) (sum_seq s j k)) (decreases j - i) =
+    if i = j - 1 then () else (sum_seq_lemma s (i + 1) j k; add_mod_assoc (FStar.Seq.index s i) (sum_seq s (i + 1) j) (sum_seq s j k))
+
+// Impure SUM
+
+
+let gpu_pts_to_slice_sum_inner
+  (#sz:nat)
+  (r: gpu_array U64.t sz)
+  (i j:nat)
+  (v: FStar.Seq.seq U64.t)
+  (s: FStar.Seq.seq U64.t)
+: slprop = gpu_pts_to_array_slice r i j s ** pure (i < j /\ j <= sz /\ FStar.Seq.length v = sz /\ FStar.Seq.length s = j - i /\ FStar.Seq.index s 0 = sum_seq v i j)
+
+let gpu_pts_to_slice_sum
+  (#sz:nat)
+  (r: gpu_array U64.t sz)
+  (i j:nat)
+  (v: FStar.Seq.seq U64.t)
+: slprop = if_ (i < j && j <= sz) (exists* s. gpu_pts_to_slice_sum_inner #sz r i j v s)
+
+// ```pulse
+// fn slice_sum_read
+//   (#sz: nat)
+//   (#r: gpu_array U64.t sz)
+//   (#i #j:nat)
+//   (#v: FStar.Seq.seq U64.t)
+//   (#_: squash (i < j /\ j <= sz /\ FStar.Seq.length v = sz))
+//   requires gpu ** gpu_pts_to_slice_sum #sz r i j v
+//   returns  result: U64.t
+//   ensures  gpu ** gpu_pts_to_slice_sum #sz r i j v ** pure (result = sum_seq v i j)
+// {
+//   unfold gpu_pts_to_slice_sum;
+//   if_elim_true _ _;
+//   with s. assert (gpu_pts_to_slice_sum_inner #sz r i j v s);
+//   unfold gpu_pts_to_slice_sum_inner;
+
+//   let ret = gpu_array_read #U64.t #sz #i #j r i;
+
+//   fold (gpu_pts_to_slice_sum_inner #sz r i j v s);
+//   if_intro_true (i < j && j <= sz) (exists* s. gpu_pts_to_slice_sum_inner #sz r i j v s);
+//   fold (gpu_pts_to_slice_sum r i j v);
+//   ret
+// }
+// ```
+
+// Barrier
+
+let barrier_pre (nth: nat) (r : gpu_array U64.t nth) (v: erased (FStar.Seq.seq U64.t)) (it tid: nat): slprop =
+  if_ (not (div_pow_2 (it + 1) tid) && (div_pow_2 it tid)) (gpu_pts_to_slice_sum r tid (min (tid + pow2 it) nth) v)
+
+let barrier_post (nth: nat) (r : gpu_array U64.t nth) (v: erased (FStar.Seq.seq U64.t)) (it tid: nat): slprop =
+  if_ (div_pow_2 (it + 1) tid) (gpu_pts_to_slice_sum r (min (tid + pow2 it) nth) (min (tid + 2 * pow2 it) nth) v)
+
+// #push-options "--debug SMTFail --split_queries always"
+// #push-options "--print_implicits"
+
+```pulse
+fn iteration
+  (nth : nat)
+  (r : gpu_array U64.t nth)
+  (b: erased (barrier nth))
+  (v: erased (FStar.Seq.seq U64.t))
+  (#_: squash (FStar.Seq.length v == nth))
+  (tid : nat{tid < nth})
+  (it: nat)
+  requires gpu
+    ** barrier_tok (barrier_pre nth r v) (barrier_post nth r v) b it tid
+    ** if_ (div_pow_2 it tid) (gpu_pts_to_slice_sum r tid (min (tid + pow2 it) nth) v)
+  ensures gpu
+    ** barrier_tok (barrier_pre nth r v) (barrier_post nth r v) b (it+1) tid
+    ** if_ (div_pow_2 (it+1) tid) (gpu_pts_to_slice_sum r tid (min (tid + pow2 (it + 1)) nth) v)
+{
+  assert (pure (FStar.Seq.length v = nth));
+
+  case_split (div_pow_2 (it + 1) tid) (if_ (div_pow_2 it tid) (gpu_pts_to_slice_sum r tid (min (tid + pow2 it) nth) v));
+  if_flatten #(div_pow_2 (it + 1) tid);
+  if_flatten #(not (div_pow_2 (it + 1) tid));
+  fold (barrier_pre nth r v it tid);
+  barrier_wait #nth #(barrier_pre nth r v) #(barrier_post nth r v) b #it #tid;
+  unfold barrier_post nth r v it tid;
+
+  div_pow_2_lemma it (it + 1) tid;
+
+  rewrite (if_ (div_pow_2 (it + 1) tid && div_pow_2 it tid)
+            (gpu_pts_to_slice_sum r tid (min (tid + pow2 it) nth) v))
+      as (if_ (div_pow_2 (it + 1) tid)
+            (gpu_pts_to_slice_sum r tid (min (tid + pow2 it) nth) v));
+
+  combine (div_pow_2 (it + 1) tid) (gpu_pts_to_slice_sum r tid (min (tid + pow2 it) nth) v) _;
+
+  if (tid % pow2 (it + 1) = 0) {
+    // if_map (fun (_: unit) -> gpu_slice_concat r (1.0R) tid (tid + pow2 it) (tid + 2 * pow2 it));
+    if_elim_true _ _;
+
+    let middle = min (tid + pow2 it) nth;
+    let end_ = min (tid + 2 * pow2 it) nth;
+
+
+    if (tid + pow2 it < nth) {
+      unfold (gpu_pts_to_slice_sum r tid middle v);
+      if_elim_true _ _;
+      unfold gpu_pts_to_slice_sum_inner;
+      unfold (gpu_pts_to_slice_sum r middle end_ v);
+      if_elim_true _ _;
+      unfold gpu_pts_to_slice_sum_inner;
+
+      let s1 = gpu_array_read #U64.t #nth #tid #middle r tid;
+      // assert (pure (s1 == sum_seq v tid middle));
+      let s2 = gpu_array_read #U64.t #nth #middle #end_ r middle;
+      // assert (pure (s2 == sum_seq v middle end_));
+      let s = U64.add_mod s1 s2;
+      sum_seq_lemma v tid middle end_;
+      // assert (pure ( s == sum_seq v tid end_ ));
+      gpu_array_write #U64.t #nth #tid #middle r tid s;
+
+      gpu_slice_concat #U64.t #nth r 1.0R tid middle end_;
+      with seq. assert (gpu_pts_to_array_slice r tid end_ seq);
+      // assert (pure (FStar.Seq.index seq 0 == s));
+      fold (gpu_pts_to_slice_sum_inner #nth r tid end_ v seq);
+      if_intro_true (tid < end_ && end_ <= nth) (exists* s. gpu_pts_to_slice_sum_inner #nth r tid end_ v s);
+      fold (gpu_pts_to_slice_sum r tid end_ v);
+      if_intro_true (div_pow_2 (it + 1) tid) (gpu_pts_to_slice_sum r tid end_ v);
+    } else {
+      unfold (gpu_pts_to_slice_sum r middle end_ v);
+      if_elim_false _ _;
+      // assert (pure (middle == end_));
+      if_intro_true (div_pow_2 (it + 1) tid) (gpu_pts_to_slice_sum r tid end_ v);
+    }
+  }
+}
+```
+
+let kpre (nth: nat) (ga1 ga2 r : gpu_array U64.t nth) (#s1 #s2: erased (FStar.Seq.seq U64.t))
+  (#_: squash ( FStar.Seq.length s1 == nth /\ FStar.Seq.length s2 == nth ))
+  (b: erased (barrier nth)) (tid:nat{tid < nth})
+  : slprop =
+    (gpu_pts_to_array #U64.t #nth ga1 #(1.0R /. Real.of_int nth) s1 **
+    gpu_pts_to_array #U64.t #nth ga2 #(1.0R /. Real.of_int nth) s2) **
+    gpu_pts_to_array1 r tid **
+    barrier_tok (barrier_pre nth r (dot s1 s2)) (barrier_post nth r (dot s1 s2)) b 0 tid
+
+let kpost (nth: nat) (ga1 ga2 r : gpu_array U64.t nth) (#s1 #s2: erased (FStar.Seq.seq U64.t))
+  (#_: squash ( FStar.Seq.length s1 == nth /\ FStar.Seq.length s2 == nth ))
+  (b: erased (barrier nth)) (tid:nat{tid < nth})
+  : slprop =
+    ((gpu_pts_to_array #U64.t #nth ga1 #(1.0R /. Real.of_int nth) s1 **
+    gpu_pts_to_array #U64.t #nth ga2 #(1.0R /. Real.of_int nth) s2) **
+    if_ (tid = 0) (gpu_pts_to_slice_sum r 0 nth (dot s1 s2))) **
+    (exists* it. barrier_tok (barrier_pre nth r (dot s1 s2)) (barrier_post nth r (dot s1 s2)) b it tid)
+
+// #set-options "--ext pulse:env_on_err=1"
 
 ```pulse
 fn kernel
-  (ga1 ga2 : gpu_array int size)
-  (r : gpu_array int size)
-  (nth : erased nat)
+  (nth : nat)
+  (ga1 ga2 : gpu_array U64.t nth)
+  (r : gpu_array U64.t nth)
+  (#s1 #s2: erased (FStar.Seq.seq U64.t))
+  (#_: squash ( FStar.Seq.length s1 == nth /\ FStar.Seq.length s2 == nth ))
+  (b: erased (barrier nth))
   (tid : nat{tid < nth})
-  requires gpu ** kpre  ga1 ga2 r nth tid
-  ensures  gpu ** kpost ga1 ga2 r nth tid
+  requires gpu ** kpre  nth ga1 ga2 r #s1 #s2 b tid
+  ensures  gpu ** kpost nth ga1 ga2 r #s1 #s2 b tid
 {
-  (**)unfold (kpre ga1 ga2 r nth tid);
+  (**)unfold (kpre nth ga1 ga2 r #s1 #s2 b tid);
 
-  (**)unfold (gpu_pts_to_array1 ga1 tid);
-  (**)gpu_pts_to_slice_ref ga1 tid (tid+1); // recall tid < size
-  let v1 = gpu_array_read #int #size #tid #(tid+1) ga1 tid;
+  (**)unfold (gpu_pts_to_array #U64.t #nth ga1 #(1.0R /. Real.of_int nth) s1);
+  let v1 = gpu_array_read #U64.t #nth #0 #nth ga1 tid #s1;
+  (**)fold (gpu_pts_to_array #U64.t #nth ga1 #(1.0R /. Real.of_int nth) s1);
 
-  (**)unfold (gpu_pts_to_array1 ga2 tid);
-  let v2 = gpu_array_read #int #size #tid #(tid+1) ga2 tid;
+  (**)unfold (gpu_pts_to_array #U64.t #nth ga2 #(1.0R /. Real.of_int nth) s2);
+  let v2 = gpu_array_read #U64.t #nth #0 #nth ga2 tid #s2;
+  (**)fold (gpu_pts_to_array #U64.t #nth ga2 #(1.0R /. Real.of_int nth) s2);
   
-  let v = v1 * v2;
+  let vm = U64.mul_mod v1 v2;
+  let dot_v = dot s1 s2;
   
   (**)unfold (gpu_pts_to_array1 r tid);
-  gpu_array_write #int #size #tid #(tid+1) r tid v;
+  gpu_array_write #U64.t #nth #tid #(tid+1) r tid vm;
   
   (* Reduction *)
-  let mut n = size / 2 <: int;
-  with vn. assert (pts_to n vn);
+  let mut n = 0 <: nat;
 
+  (**)with s. assert (gpu_pts_to_array_slice r tid (tid+1) s);
+  (**)fold (gpu_pts_to_slice_sum_inner #nth r tid (tid+1) dot_v s);
+  (**)if_intro_true (tid < tid + pow2 0 && tid + pow2 0 <= nth) (exists* s. gpu_pts_to_slice_sum_inner #nth r tid (tid + pow2 0) dot_v s);
+  (**)fold (gpu_pts_to_slice_sum r tid (tid + pow2 0) dot_v);
+  (**)if_intro_true (div_pow_2 0 tid) (gpu_pts_to_slice_sum r tid (tid + pow2 0) dot_v);
 
-  assume_ (if tid < size / 2 then (exists* s. gpu_pts_to_array_slice r (tid+size/2) (tid+size/2+1) s) else emp);
-
-  admit();
-
-  rewrite (exists* s. gpu_pts_to_array_slice r tid (tid+1) s)
-       as (if tid < vn then (exists* s. gpu_pts_to_array_slice r tid (tid+1) s) else emp);
-
-  let a = 123;
-  while (let vn = !n; (vn > 1))
-    invariant b. exists* vn.
+  while (let it = !n; (pow2 it < nth))
+    invariant c.
+    exists* (it:nat).
       gpu **
-      (if tid < vn
-       then (exists* s. gpu_pts_to_array_slice r tid (tid+1) s)
-       else emp) **
-      pts_to n vn **
-      pure (vn <= size / 2 /\ b == (vn > 1))
+      pts_to n it **
+      barrier_tok #nth (barrier_pre nth r dot_v) (barrier_post nth r dot_v) b it tid **
+      if_ (div_pow_2 it tid) (gpu_pts_to_slice_sum r tid (min (tid + pow2 it) nth) dot_v) **
+      pure (c == (pow2 it < nth))
   {
-    let vn = !n;
-    if (tid < vn) {
-      (**)rewrite
-             (if tid < vn then (exists* s. gpu_pts_to_array_slice r tid (tid+1) s) else emp)
-          as (exists* s. gpu_pts_to_array_slice r tid (tid+1) s);
-      let vl = gpu_array_read #int #size #tid #(tid+1) r tid;
-      assume_ (exists* s. gpu_pts_to_array_slice r (tid+vn) (tid+vn+1) s);
-      assume_ (pure (tid + vn < size));
-      let vr = gpu_array_read #int #size #(tid+vn) #(tid+vn+1) r (tid + vn);
-      gpu_array_write #int #size #tid #(tid+1) r tid (vl + vr);
-      n := vn / 2;
-      ()
-    } else {
-      n := vn / 2;
-      assert (if tid < (vn / 2) then (exists* s. gpu_pts_to_array_slice r tid (tid+1) s) else emp);
-      (* sync_threads() *)
-      ()
-    };
+    let it = !n <: nat;
+    iteration nth r b dot_v tid it;
+    n := it + 1;
   };
+  
+  (**)let it = !n;
+  (**)mod_lemma tid (pow2 it);
+  // assert (pure (pow2 it >= nth /\ tid < nth /\ (div_pow_2 it tid) == (tid = 0)));
 
-  (**)fold (gpu_pts_to_array1 r tid);
-  (**)fold (gpu_pts_to_array1 ga1 tid);
-  (**)fold (gpu_pts_to_array1 ga2 tid);
-  (**)fold (kpost ga1 ga2 r nth tid);
+  // rewrite (if_ (div_pow_2 (reveal it) tid) (gpu_pts_to_slice_sum r tid (min (tid + pow2 (reveal it)) nth) dot_v))
+  //     as  (if_ (tid = 0) (gpu_pts_to_slice_sum r tid nth dot_v));
+
+  if (tid = 0) {
+    (**)if_elim_true _ _;
+    (**)if_intro_true (tid = 0) (gpu_pts_to_slice_sum r 0 nth dot_v);
+    (**)fold (kpost nth ga1 ga2 r #s1 #s2 b tid);
+  } else {
+    (**)fold (kpost nth ga1 ga2 r #s1 #s2 b tid);
+  };
+}
+```
+
+let shared_array (#nth : nat { nth <> 0 }) (ga : gpu_array U64.t nth) (#v: FStar.Seq.seq U64.t { FStar.Seq.length v == nth }) (_: nat): slprop =
+  gpu_pts_to_array ga #(1.0R /. Real.of_int nth) v
+
+```pulse
+fn share_array
+  (#nth : nat { nth <> 0 })
+  (ga : gpu_array U64.t nth)
+  (#v: erased (FStar.Seq.seq U64.t) { reveal (FStar.Seq.length v) == nth })
+  requires gpu_pts_to_array ga #1.0R v
+  ensures  bigstar 0 nth (shared_array #nth ga #v)
+{
+  rewrite gpu_pts_to_array ga #1.0R v
+    as gpu_pts_to_array ga #(1.0R /. of_int 1) v;
+  admit();
 }
 ```
 
 ```pulse
-fn main (_:unit)
-  requires cpu
-  ensures  cpu
+fn gather_array
+  (#nth : nat { nth <> 0 })
+  (ga : gpu_array U64.t nth)
+  (#v: erased (FStar.Seq.seq U64.t) { reveal (FStar.Seq.length v) == nth })
+  requires bigstar 0 nth (shared_array #nth ga #v)
+  ensures  gpu_pts_to_array ga #1.0R v
 {
-  let a1 = A.alloc 0 (SZ.uint_to_t size);
-  let a2 = A.alloc 0 (SZ.uint_to_t size);
-  let ar = A.alloc 0 (SZ.uint_to_t size);
+  admit();
+}
+```
+
+```pulse
+ghost fn barrier_proof
+  (nth : nat)
+  (r: gpu_array U64.t nth)
+  (v: FStar.Seq.seq U64.t { FStar.Seq.length v == nth })
+  (it: nat)
+  requires bigstar 0 nth ((barrier_pre nth r v) it)
+  ensures  bigstar 0 nth ((barrier_post nth r v) it)
+{
+  // TODO: proof
+  admit()
+}
+```
+
+// #push-options "--print_implicits"
+
+
+```pulse
+ghost fn bigstar_if
+  (n m x: nat)
+  (p: slprop)
+  (#_: squash (n <= x /\ x < m))
+  requires bigstar n m (fun i -> if_ (i = x) p)
+  ensures  p
+{
+  admit()
+}
+```
+
+```pulse
+fn main
+  (a1 a2: array U64.t)
+  (v1 v2: erased (Seq.Base.seq U64.t))
+  (#_: squash (Seq.length v1 = size /\ Seq.length v2 = size))
+  requires cpu ** A.pts_to a1 v1 ** A.pts_to a2 v2
+  returns dp: U64.t
+  ensures  cpu ** A.pts_to a1 v1 ** A.pts_to a2 v2 ** pure (dp == sum_seq (dot v1 v2) 0 size)
+{
+  let ar = A.alloc #U64.t 0UL (SZ.uint_to_t size);
 
   let mut i = 0sz;
 
-  while (let v = !i; (SZ.v v < size))
-     invariant b.
-       exists* v. pts_to i v **
-       (exists* s. A.pts_to a1 s ** pure (Seq.length s == size)) **
-       (exists* s. A.pts_to a2 s ** pure (Seq.length s == size)) **
-       pure (b == (SZ.v v < size))
-  {
-    let v = !i;
-    a1.(v) <- SZ.v v;
-    a2.(v) <- SZ.v v;
-    i := SZ.add v 1sz;
-    ()
-  };
+  // while (let v = !i; (SZ.v v < size))
+  //    invariant b.
+  //      exists* v. pts_to i v **
+  //      (exists* s. A.pts_to a1 s ** pure (Seq.length s == size)) **
+  //      (exists* s. A.pts_to a2 s ** pure (Seq.length s == size)) **
+  //      pure (b == (SZ.v v < size))
+  // {
+  //   let v = !i;
+  //   a1.(v) <- SZ.v v;
+  //   a2.(v) <- SZ.v v;
+  //   i := SZ.add v 1sz;
+  //   ()
+  // };
 
-  let ga1 = gpu_array_alloc #int size;
-  let ga2 = gpu_array_alloc #int size;
+  let ga1 = gpu_array_alloc #U64.t size;
+  let ga2 = gpu_array_alloc #U64.t size;
 
   GPU.Array.gpu_memcpy_host_to_device a1 ga1;
   GPU.Array.gpu_memcpy_host_to_device a2 ga2;
   
-  let gr = gpu_array_alloc #int size;
+  let gr = gpu_array_alloc #U64.t size;
 
   // Slicing the arrays
-  (**)gpu_array_slice_1_underspec ga1;
-  (**)gpu_array_slice_1_underspec ga2;
+  (**)share_array ga1;
+  (**)share_array ga2;
   (**)gpu_array_slice_1_underspec gr;
-  
+
+  let b = mk_barrier size (barrier_pre size gr (dot v1 v2)) (barrier_post size gr (dot v1 v2)) (barrier_proof size gr (dot v1 v2));
+
   // Boring combination of resources
-  (**)bigstar_zip 0 size (gpu_pts_to_array1 ga1) (gpu_pts_to_array1 ga2);
+  (**)bigstar_zip 0 size (shared_array ga1) (shared_array ga2);
   (**)bigstar_zip 0 size _ (gpu_pts_to_array1 gr);
+  (**)bigstar_zip 0 size _ (barrier_tok (barrier_pre size gr (dot v1 v2)) (barrier_post size gr (dot v1 v2)) b 0);
   (**)rewrite
     (bigstar 0 size
-      (fun i -> (gpu_pts_to_array1 ga1 i **
-                 gpu_pts_to_array1 ga2 i) **
-                 gpu_pts_to_array1 gr i))
+      (fun i -> ((shared_array #size ga1 #v1 i **
+                 shared_array #size ga2 #v2 i) **
+                 gpu_pts_to_array1 gr i) **
+                 barrier_tok (barrier_pre size gr (dot v1 v2)) (barrier_post size gr (dot v1 v2)) b 0 i))
   as
-    (bigstar 0 size (fun i -> kpre ga1 ga2 gr size i));
+    (bigstar 0 size (fun i -> kpre size ga1 ga2 gr #v1 #v2 b i));
   (**)bigstar_uneta ();
-  
-  launch_kernel_n size (kernel ga1 ga2 gr size);
-  
+
+  launch_kernel_n size #(kpre size ga1 ga2 gr #v1 #v2 b) #(kpost size ga1 ga2 gr #v1 #v2 b) (kernel size ga1 ga2 gr #v1 #v2 b);
+
   (**)bigstar_eta ();
-  (**)rewrite
-    (bigstar 0 size (fun i -> kpost ga1 ga2 gr size i))
-  as
-    (bigstar 0 size
-      (fun i -> gpu_pts_to_array1 ga1 i **
-                gpu_pts_to_array1 ga2 i **
-                gpu_pts_to_array1 gr i));
+  // TODO:
+  (**)drop_
+        (bigstar 0 size (fun i -> kpost size ga1 ga2 gr #v1 #v2 b i));
+  let it = 10;
+  (**)assume_
+        (bigstar 0 size
+          (fun i -> ((gpu_pts_to_array #U64.t #size ga1 #(1.0R /. Real.of_int size) v1 **
+                    gpu_pts_to_array #U64.t #size ga2 #(1.0R /. Real.of_int size) v2) **
+                    if_ (i = 0) (gpu_pts_to_slice_sum gr 0 size (dot v1 v2))) **
+                    barrier_tok (barrier_pre size gr (dot v1 v2)) (barrier_post size gr (dot v1 v2)) b it i
+        ));
+  
+  (**)bigstar_unzip 0 size _ _;
   (**)bigstar_unzip 0 size _ _;
   (**)bigstar_unzip 0 size _ _;
   
-  // Unslicing
-  (**)gpu_array_unslice_1_underspec ga1;
-  (**)gpu_array_unslice_1_underspec ga2;
-  (**)gpu_array_unslice_1_underspec gr;
-  
+  (**)bigstar_uneta () #0 #size #(shared_array #size ga1 #v1);
+  gather_array ga1;
+  (**)bigstar_uneta () #0 #size #(shared_array #size ga2 #v2);
+  gather_array ga2;
+
+  drop_barrier #size #(barrier_pre size gr (dot v1 v2)) #(barrier_post size gr (dot v1 v2)) #b #it;
+
+  bigstar_if 0 size 0 (gpu_pts_to_slice_sum #size gr 0 size (dot v1 v2)) #();
+  unfold gpu_pts_to_slice_sum;
+  if_elim_true _ _;
+  unfold gpu_pts_to_slice_sum_inner;
+  with res. assert (gpu_pts_to_array_slice gr 0 size res);
+  fold (gpu_pts_to_array #U64.t #size gr #1.0R res);
+
+  // TODO: don't copy whole array
   GPU.Array.gpu_memcpy_device_to_host ar gr;
 
-  i := 0sz;
-  let mut psum = 0;
-  while (let v = !i; (SZ.v v < size))
-     invariant b. exists* vi vpsum.
-       pts_to i vi **
-       pts_to psum vpsum  **
-       (exists* s. A.pts_to ar s ** pure (Seq.length s == size)) **
-       pure (b == (SZ.v vi < size))
-  {
-    let vi = !i;
-    let ri = ar.(vi);
-    let vpsum = !psum;
-    psum := vpsum + ri;
-    i := SZ.add vi 1sz;
-  };
-  
-  A.free a1;
-  A.free a2;
-  A.free ar;
   gpu_array_free ga1;
   gpu_array_free ga2;
   gpu_array_free gr;
 
-  ()
+  let dp = ar.(0sz);
+  A.free ar;
+  dp
 }
 ```
