src/lib/GPU.Conditional.fst
@@ -1,0 +1,170 @@
+module GPU.Conditional
+
+open Pulse.Lib.Pervasives
+open FStar.Tactics.V2
+
+let if_ (b: bool) (p: slprop): slprop = (cond b p emp)
+
+// INTRODUCTION and ELIMINATION RULES
+
+```pulse
+ghost fn if_intro_true (b: bool) (p: slprop)
+  requires p ** (pure b)
+  ensures  if_ b p
+{
+  rewrite p as if_ b p;
+}
+```
+
+```pulse
+ghost fn if_intro_false (b: bool) (p: slprop)
+  requires emp ** (pure (not b))
+  ensures  if_ b p
+{
+  rewrite emp as if_ b p;
+}
+```
+
+```pulse
+ghost fn if_elim_true (b: bool) (p: slprop)
+  requires if_ b p ** (pure b)
+  ensures  p
+{
+  unfold if_ b p;
+  rewrite (if b then p else emp) as p;
+}
+```
+
+```pulse
+ghost fn if_elim_false (b: bool) (p: slprop)
+  requires if_ b p ** (pure (not b))
+  ensures  emp
+{
+  unfold if_ b p;
+  rewrite (if b then p else emp) as emp;
+}
+```
+
+// SPLIT and JOIN RULES
+
+```pulse
+ghost fn case_split (b: bool) (p: slprop)
+  requires p
+  ensures  if_ b p ** if_ (not b) p
+{
+  if b {
+    if_intro_true b p;
+    if_intro_false (not b) p;
+  } else {
+    if_intro_true (not b) p;
+    if_intro_false b p;
+  }
+}
+```
+
+```pulse
+ghost fn case_join (b: bool) (p: slprop)
+  requires if_ b p ** if_ (not b) p
+  ensures  p
+{
+  if b {
+    if_elim_true b p;
+    if_elim_false (not b) p;
+  } else {
+    if_elim_true (not b) p;
+    if_elim_false b p;
+  
+  }
+}
+```
+
+// COMBINE and SPLIT RULES
+
+```pulse
+ghost fn combine (b: bool) (p1 p2: slprop)
+  requires if_ b p1 ** if_ b p2
+  ensures  if_ b (p1 ** p2)
+{
+  if b {
+    if_elim_true b p1;
+    if_elim_true b p2;
+    if_intro_true b (p1 ** p2);
+  } else {
+    if_elim_false b p1;
+    if_elim_false b p2;
+    if_intro_false b (p1 ** p2);
+  }
+}
+```
+
+```pulse
+ghost fn split (b: bool) (p1 p2: slprop)
+  requires if_ b (p1 ** p2)
+  ensures  if_ b p1 ** if_ b p2
+{
+  if b {
+    if_elim_true b (p1 ** p2);
+    if_intro_true b p1;
+    if_intro_true b p2;
+  } else {
+    if_elim_false b (p1 ** p2);
+    if_intro_false b p1;
+    if_intro_false b p2;
+  }
+}
+```
+
+// MAP
+
+```pulse
+ghost fn if_map (#b: bool) (#p #q: slprop) (f: unit -> (stt_ghost unit emp_inames (p) (fun _ -> q)))
+  requires if_ b p
+  ensures  if_ b q
+{
+  if b {
+    if_elim_true b p;
+    f ();
+    if_intro_true b q;
+  } else {
+    if_elim_false b p;
+    if_intro_false b q;
+  }
+}
+```
+
+```pulse
+ghost fn if_flatten (#b1 #b2: bool) (#p: slprop)
+  requires if_ b1 (if_ b2 p)
+  ensures  if_ (b1 && b2) p
+{
+  if b1 {
+    if_elim_true b1 (if_ b2 p);
+    if b2 {
+      if_elim_true b2 p;
+      if_intro_true (b1 && b2) p;
+    } else {
+      if_elim_false b2 p;
+      if_intro_false (b1 && b2) p;
+    }
+  } else {
+    if_elim_false b1 (if_ b2 p);
+    if_intro_false (b1 && b2) p;
+  }
+}
+```
+
+// REWRITE
+
+```pulse
+ghost fn if_rewrite (#b: bool) (#p1 p2: slprop) (#e: (squash b -> squash (p1 == p2)))
+  requires if_ b p1
+  ensures  if_ b p2
+{
+  if b {
+    e ();
+    rewrite each p1 as p2;
+  } else {
+    ()
+  }
+}
+```
